Prefix(:=<http://www.ease-crc.org/ont/SOMA.owl#>)
Prefix(dc:=<http://purl.org/dc/elements/1.1/>)
Prefix(owl:=<http://www.w3.org/2002/07/owl#>)
Prefix(rdf:=<http://www.w3.org/1999/02/22-rdf-syntax-ns#>)
Prefix(xml:=<http://www.w3.org/XML/1998/namespace>)
Prefix(xsd:=<http://www.w3.org/2001/XMLSchema#>)
Prefix(SOMA:=<http://www.ease-crc.org/ont/SOMA.owl#>)
Prefix(rdfs:=<http://www.w3.org/2000/01/rdf-schema#>)


Ontology(<http://www.ease-crc.org/ont/SOMA-IO.owl>
Import(<http://www.ease-crc.org/ont/SOMA.owl>)

Declaration(Class(SOMA:ComputationalAgent))
Declaration(Class(SOMA:DigitalData))
Declaration(Class(SOMA:DigitalObject))
Declaration(Class(SOMA:FaultySoftware))
Declaration(Class(SOMA:IncompatibleSoftware))
Declaration(Class(SOMA:SoftwareImplementation))
Declaration(Class(SOMA:SoftwarePackage))
Declaration(Class(SOMA:SoftwareType))
Declaration(Class(SOMA:UnavailableSoftware))
Declaration(Class(<http://www.ontologydesignpatterns.org/ont/dul/IOLite.owl#DigitalResource>))



############################
#   Classes
############################

# Class: <http://www.ease-crc.org/ont/SOMA.owl#ComputationalAgent> (Computational agent)

AnnotationAssertion(rdfs:comment SOMA:ComputationalAgent "An agent that is implemented in software.")
AnnotationAssertion(rdfs:label SOMA:ComputationalAgent "Computational agent")
EquivalentClasses(SOMA:ComputationalAgent ObjectIntersectionOf(SOMA:SoftwareImplementation <http://www.ontologydesignpatterns.org/ont/dul/DUL.owl#Agent>))

# Class: <http://www.ease-crc.org/ont/SOMA.owl#DigitalData> (Digital data)

AnnotationAssertion(rdfs:comment SOMA:DigitalData "An information realization of quantitative data.")
AnnotationAssertion(rdfs:label SOMA:DigitalData "Digital data")
SubClassOf(SOMA:DigitalData <http://www.ontologydesignpatterns.org/ont/dul/IOLite.owl#DigitalResource>)

# Class: <http://www.ease-crc.org/ont/SOMA.owl#DigitalObject> (Digital object)

AnnotationAssertion(rdfs:comment SOMA:DigitalObject "An information realization with object character. e.g. a software agent etc.")
AnnotationAssertion(rdfs:label SOMA:DigitalObject "Digital object")
SubClassOf(SOMA:DigitalObject <http://www.ontologydesignpatterns.org/ont/dul/DUL.owl#Object>)
SubClassOf(SOMA:DigitalObject <http://www.ontologydesignpatterns.org/ont/dul/IOLite.owl#DigitalResource>)

# Class: <http://www.ease-crc.org/ont/SOMA.owl#FaultySoftware> (Faulty software)

AnnotationAssertion(rdfs:comment SOMA:FaultySoftware "A description of a situation where some software has a bug.")
AnnotationAssertion(rdfs:label SOMA:FaultySoftware "Faulty software"@en)
SubClassOf(SOMA:FaultySoftware SOMA:SoftwareDiagnosis)

# Class: <http://www.ease-crc.org/ont/SOMA.owl#IncompatibleSoftware> (Incompatible software)

AnnotationAssertion(rdfs:comment SOMA:IncompatibleSoftware "A description of a situation where two software systems are incompatible with each other.")
AnnotationAssertion(rdfs:label SOMA:IncompatibleSoftware "Incompatible software"@en)
SubClassOf(SOMA:IncompatibleSoftware SOMA:SoftwareDiagnosis)

# Class: <http://www.ease-crc.org/ont/SOMA.owl#SoftwareImplementation> (Software implementation)

AnnotationAssertion(rdfs:comment SOMA:SoftwareImplementation "An information realization in form of a executable computer program.")
AnnotationAssertion(rdfs:label SOMA:SoftwareImplementation "Software implementation")
SubClassOf(SOMA:SoftwareImplementation SOMA:DigitalObject)

# Class: <http://www.ease-crc.org/ont/SOMA.owl#SoftwarePackage> (Software package)

AnnotationAssertion(rdfs:comment SOMA:SoftwarePackage "A structured archive of software that also often contains data needed to run the software, and scripts to build and configure the software.")
AnnotationAssertion(rdfs:label SOMA:SoftwarePackage "Software package")
SubClassOf(SOMA:SoftwarePackage SOMA:DigitalObject)

# Class: <http://www.ease-crc.org/ont/SOMA.owl#SoftwareType> (Software type)

AnnotationAssertion(rdfs:comment SOMA:SoftwareType "A concept that classifies software objects.")
AnnotationAssertion(rdfs:label SOMA:SoftwareType "Software type")
SubClassOf(SOMA:SoftwareType <http://www.ontologydesignpatterns.org/ont/dul/DUL.owl#Role>)
SubClassOf(SOMA:SoftwareType ObjectAllValuesFrom(<http://www.ontologydesignpatterns.org/ont/dul/DUL.owl#classifies> SOMA:SoftwareImplementation))

# Class: <http://www.ease-crc.org/ont/SOMA.owl#UnavailableSoftware> (Unavailable software)

AnnotationAssertion(rdfs:comment SOMA:UnavailableSoftware "A description of a situation where some software dependency is not available.")
AnnotationAssertion(rdfs:label SOMA:UnavailableSoftware "Unavailable software"@en)
SubClassOf(SOMA:UnavailableSoftware SOMA:SoftwareDiagnosis)


)